theories/zoo/iris/bi/big_op.v
@@ -1,3 +1,6 @@
+From stdpp Require Import
+  fin_sets.
+
 From iris.bi Require Export
   big_op.
 
@@ -947,4 +950,53 @@ Section bi.
       rewrite !big_opM_map_to_list map_to_list_kmap big_sepL_fmap //.
     Qed.
   End big_sepM.
+
+  Section big_sepS.
+    Context `{Countable K}.
+
+    Implicit Types s : gset K.
+    Implicit Types P : PROP.
+    Implicit Types Φ : K → PROP.
+
+    Lemma big_sepS_impl_thread {Φ1} P Φ2 s :
+      ([∗ set] x ∈ s, Φ1 x) -∗
+      P -∗
+      □ (
+        ∀ x,
+        ⌜x ∈ s⌝ →
+        Φ1 x -∗
+        P -∗
+          Φ2 x ∗
+          P
+      ) -∗
+        ([∗ set] x ∈ s, Φ2 x) ∗
+        P.
+    Proof.
+      rewrite !big_sepS_elements.
+      iIntros "Hs HP #HΦ".
+      iApply (big_sepL_impl_thread with "Hs HP"). iIntros "!>" (k x Hx%elem_of_list_lookup_2%elem_of_elements) "HΦ1 HP".
+      iApply ("HΦ" with "[//] HΦ1 HP").
+    Qed.
+    Lemma big_sepS_impl_thread_fupd `{!BiFUpd PROP} {Φ1} P Φ2 s E :
+      ([∗ set] x ∈ s, Φ1 x) -∗
+      P -∗
+      □ (
+        ∀ x,
+        ⌜x ∈ s⌝ →
+        Φ1 x -∗
+        P -∗
+          |={E}=>
+          Φ2 x ∗
+          P
+      ) -∗
+        |={E}=>
+        ([∗ set] x ∈ s, Φ2 x) ∗
+        P.
+    Proof.
+      rewrite !big_sepS_elements.
+      iIntros "Hs HP #HΦ".
+      iApply (big_sepL_impl_thread_fupd with "Hs HP"). iIntros "!>" (k x Hx%elem_of_list_lookup_2%elem_of_elements) "HΦ1 HP".
+      iApply ("HΦ" with "[//] HΦ1 HP").
+    Qed.
+  End big_sepS.
 End bi.
