theories/zoo/program_logic/adequacy.v
@@ -15,17 +15,21 @@ Implicit Types e : expr.
 Implicit Types v : val.
 Implicit Types σ : state.
 
-Definition zoo_adequacy `{zoo_Gpre : !ZooGpre Σ} e σ v :
+Definition zoo_adequacy `{zoo_Gpre : !ZooGpre Σ} e σ v cnt :
   σ.(state_locals) = [v] →
+  σ.(state_heap) !! zoo_counter = Some (ValNat cnt) →
   ( ∀ `{zoo_G : !ZooG Σ},
+    ( [∗ map] l ↦ v ∈ delete zoo_counter σ.(state_heap),
+      l ↦ v
+    ) -∗
     0 ↦ₗ v -∗
     WP e ∶ 0 {{ v, True }}
   ) →
   safe ([e], σ).
 Proof.
-  intros Hlocals Hwp.
+  intros Hlocals Hcounter Hwp.
   apply: wp_adequacy => // Hinv_G κs.
-  iMod (zoo_init' σ v κs) as "(%zoo_G & Hσ & Htid)"; first done.
-  iExists zoo_state_interp. repeat iExists _. iFrame.
-  iApply (Hwp (Build_ZooG _ _) with "Htid").
+  iMod (zoo_init' σ v cnt κs) as "(%zoo_G & <- & Hσ & Hheap & Hlocals)"; [done.. |].
+  iExists zoo_state_interp, (λ _, True)%I, (λ _, True)%I. iFrame.
+  iApply (Hwp with "Hheap Hlocals").
 Qed.
