theories/zoo/program_logic/counter.v
@@ -1,0 +1,80 @@
+From iris.base_logic Require Import
+  lib.invariants.
+
+From zoo Require Import
+  prelude.
+From zoo.iris.bi Require Import
+  big_op.
+From zoo.iris.base_logic Require Import
+  lib.mono_list.
+From zoo.language Require Import
+  notations.
+From zoo.program_logic Require Export
+  wp.
+From zoo.diaframe Require Import
+  diaframe.
+From zoo Require Import
+  options.
+
+Definition zoo_counter_incr : val :=
+  fun: <> =>
+    FAA (#zoo_counter).[contents] #1.
+
+Section zoo_G.
+  Context `{zoo_G : !ZooG Σ}.
+
+  Definition zoo_counter_at :=
+    mono_list_at (mono_list_G := zoo_G_counter_G) zoo_counter_name.
+
+  #[global] Instance zoo_counter_at_persistent id v :
+    Persistent (zoo_counter_at id v).
+  Proof.
+    apply _.
+  Qed.
+
+  Lemma zoo_counter_at_agree id v1 v2 :
+    zoo_counter_at id v1 -∗
+    zoo_counter_at id v2 -∗
+    ⌜v1 = v2⌝.
+  Proof.
+    apply mono_list_at_agree.
+  Qed.
+
+  Lemma zoo_counter_incr_spec ids v :
+    {{{
+      [∗ set] id ∈ ids,
+        ∃ v,
+        zoo_counter_at id v
+    }}}
+      zoo_counter_incr ()
+    {{{ id,
+      RET #id;
+      zoo_counter_at id v ∗
+      ⌜set_Forall (.≠ id) ids⌝
+    }}}.
+  Proof.
+    iIntros "%Φ Hids HΦ".
+
+    iApply wp_state_interp. iIntros "%nt %σ %κs Hσ !>".
+    iDestruct (state_interp_counter_inv with "Hσ") as "#Hinv".
+    iFrame.
+
+    wp_rec.
+    wp_pures.
+
+    iInv "Hinv" as "(%cnt & %vs & Hcounter & Hauth & ><-)".
+    wp_faa.
+    iAssert ⌜set_Forall (.≠ length vs) ids⌝%I as "%Hids".
+    { iApply big_sepS_pure.
+      iDestruct (big_sepS_impl_thread with "Hids Hauth []") as "($ & _)". iIntros "!> %id _ (%w & Hat) Hauth".
+      iDestruct (mono_list_at_valid with "Hauth Hat") as %Hid%lookup_lt_Some.
+      iSteps.
+    }
+    iMod (mono_list_update_snoc v with "Hauth") as "Hauth".
+    iDestruct (mono_list_at_get with "Hauth") as "#Hat".
+    { apply list_lookup_middle. done. }
+    iSteps. iPureIntro. rewrite length_app /=. lia.
+  Qed.
+End zoo_G.
+
+#[global] Opaque zoo_counter_at.
